Cleaned-up example code. Added "hide" tactic

Tactic/Examples/GodelT_norm/GodelT_norm(setoid).lean
@@ -1,4 +1,4 @@
-import Mathlib.Tactic
+import Tactic.setoidRw
 
 -- From: https://cs.ioc.ee/ewscs/2009/dybjer/mainPalmse-revised.pdf
 
@@ -36,9 +36,8 @@ inductive convr : Π {α : Ty}, (Exp α) → (Exp α) → Prop
 | recN_succ {α : Ty} {n : Exp Nat} {e : Exp α} {f : Exp (Nat ⇒' α ⇒' α)}
         : convr (recN ⬝ e ⬝ f ⬝ (succ ⬝ n)) (f ⬝ n ⬝ (recN ⬝ e ⬝ f ⬝ n))
 
-
 -- Setoid instance here:
-instance ExpClass.Setoid : Setoid (Exp α) :=
+instance convr_Setoid : Setoid (Exp α) :=
   { r := convr
     iseqv :=
       { refl := λ _ => convr.refl
@@ -47,39 +46,6 @@ instance ExpClass.Setoid : Setoid (Exp α) :=
       }
   }
 
-def ExpClass α := Quotient (@ExpClass.Setoid α)
-
-lemma ExpClass.def {e1 e2 : Exp α} :
-  convr e1 e2 ↔ (⟦e1⟧ : ExpClass α) = ⟦e2⟧ :=
-  by
-  apply Iff.intro
-  exact fun a => Quotient.sound a
-  exact fun a => Quotient.exact a
-
-lemma ExpClass.K : (⟦K ⬝ x ⬝ y⟧ : ExpClass α) = ⟦x⟧ := ExpClass.def.mp convr.K
-
-lemma ExpClass.S : (⟦S ⬝ x ⬝ y ⬝ z⟧ : ExpClass α) = ⟦x ⬝ z ⬝ (y ⬝ z)⟧ := ExpClass.def.mp convr.S
-
--- In Sozeau's notation:
--- Proper ( ≈ ++> ≈ ++> ≈ ) app
-lemma ExpClass.app : (⟦a⟧ : ExpClass (β ⇒' α)) = ⟦b⟧ → (⟦c⟧ : ExpClass β) = ⟦d⟧ →  (⟦a ⬝ c⟧ : ExpClass α) = ⟦b ⬝ d⟧
-  :=
-  by
-  rewrite [← ExpClass.def, ← ExpClass.def, ← ExpClass.def]
-  exact fun a_1 a_2 => convr.app a_1 a_2
-
-lemma ExpClass.app_arg : (⟦c⟧ : ExpClass β) = ⟦d⟧ →  (⟦a ⬝ c⟧ : ExpClass α) = ⟦a ⬝ d⟧
-  := fun a_1 => ExpClass.app rfl a_1
-
-lemma ExpClass.app_fun : (⟦a⟧ : ExpClass (β ⇒' α)) = ⟦b⟧ →  (⟦a ⬝ c⟧ : ExpClass α) = ⟦b ⬝ c⟧
-  := fun a_1 => ExpClass.app a_1 rfl
-
-
-
-lemma ExpClass.recN_zero : (⟦recN ⬝ e ⬝ f ⬝ zero⟧ : ExpClass α) = ⟦e⟧ := ExpClass.def.mp convr.recN_zero
-
-lemma ExpClass.recN_succ : (⟦recN ⬝ e ⬝ f ⬝ (succ ⬝ n)⟧ : ExpClass α) = ⟦f ⬝ n ⬝ (recN ⬝ e ⬝ f ⬝ n)⟧ := ExpClass.def.mp convr.recN_succ
-
 
 def Ty_inter : Ty → Type
 | Ty.Nat => ℕ
@@ -87,27 +53,21 @@ def Ty_inter : Ty → Type
 | arrow a b => Exp (a ⇒' b) × (Ty_inter a → Ty_inter b)
 
 
+
+def numeral : ℕ → Exp Ty.Nat
+| 0 => zero
+
+| n+1 => succ ⬝ (numeral n)
+
+
+def reify (α : Ty) (e : Ty_inter α) : Exp α :=
+  match α,e with
+  | Ty.Nat, e            => numeral e
+
+  | Ty.arrow α β, (c, f) => c
+
+
 def appsem {a b : Ty} (t : Ty_inter (a ⇒' b)) (e' : Ty_inter a) : Ty_inter b := (t.snd e')
-
-def reify (a : Ty) (e : Ty_inter a) : Exp a :=
-/-
-  match a with
-| Ty.Nat =>
-  match e with
-  | (0 : ℕ)    => zero
-  | n+1         => succ ⬝ (reify Ty.Nat n)
-
-| Ty.arrow a b =>
-  match e with
-  | (c, f) => c
--/
-by
-  cases a
-  case Nat =>
-    induction e
-    case zero           => exact zero
-    case succ _ reify_n => exact (succ ⬝ reify_n)
-  case arrow a b        => exact e.fst
 
 
 def Exp_inter (a : Ty) : (e : Exp a) → Ty_inter a
@@ -171,31 +131,34 @@ lemma convr_R_iff : ∀ e e', convr e e' → (R α e ↔ R α e') :=
     apply Iff.intro
     · intro a_r_nbe
       -- Translate "convr a b" to "⟦a⟧ = ⟦b⟧":
-      replace a_r_b := ExpClass.def.mp a_r_b; replace a_r_nbe := ExpClass.def.mp a_r_nbe
-      apply ExpClass.def.mpr
+      have soundness' := @soundness
+      translate `convr `convr_Setoid
+      hide soundness'
       -- b ~ a ~ nbe a = nbe b
       -- "rewrite [← a_r_b, a_r_nbe, soundness a_r_b]"
-      rw [← a_r_b, a_r_nbe, soundness $ ExpClass.def.mpr a_r_b]
+      rw [← a_r_b, a_r_nbe, soundness' a_r_b]
     · intro b_r_nbe
       -- Translate "convr a b" to "⟦a⟧ = ⟦b⟧":
-      replace a_r_b := ExpClass.def.mp a_r_b; replace b_r_nbe := ExpClass.def.mp b_r_nbe
-      apply ExpClass.def.mpr
+      have soundness' := @soundness
+      translate `convr `convr_Setoid
+      hide soundness'
       -- a ~ b ~ nbe b = nbe a
       -- "rewrite [a_r_b, b_r_nbe, ← soundness a_r_b]"
-      rw [a_r_b, b_r_nbe, ← soundness $ ExpClass.def.mpr a_r_b]
+      rw [a_r_b, b_r_nbe, ← soundness' a_r_b]
 
-  · rename_i α β _ βIH
+  · rename_i α β αIH βIH; clear αIH
     intros f1 f2 f1_r_f2
     apply Iff.intro
     · intro R_f1
       apply And.intro
       · have f1_r_nbe := R_convr_nbe R_f1; clear R_f1
         -- Translate "convr a b" to "⟦a⟧ = ⟦b⟧":
-        replace f1_r_f2 := ExpClass.def.mp f1_r_f2; replace f1_r_nbe := ExpClass.def.mp f1_r_nbe
-        apply ExpClass.def.mpr
+        have soundness' := @soundness
+        translate `convr `convr_Setoid
+        hide soundness'
         -- f2 ~ f1 ~ nbe f1 = nbe f2
         -- "rewrite [← f1_r_f2, f1_r_nbe, soundness f1_r_f2]"
-        rw [← f1_r_f2, f1_r_nbe, soundness $ ExpClass.def.mpr f1_r_f2]
+        rw [← f1_r_f2, f1_r_nbe, soundness' f1_r_f2]
       · intro e' Re'
         rewrite [← βIH (f1 ⬝ e') (f2 ⬝ e') (f1_r_f2.app convr.refl)]
         rcases R_f1 with ⟨_, h0⟩
@@ -205,37 +168,17 @@ lemma convr_R_iff : ∀ e e', convr e e' → (R α e ↔ R α e') :=
       apply And.intro
       · have f2_r_nbe := R_convr_nbe R_f2; clear R_f2
         -- Translate "convr a b" to "⟦a⟧ = ⟦b⟧":
-        replace f1_r_f2 := ExpClass.def.mp f1_r_f2; replace f2_r_nbe := ExpClass.def.mp f2_r_nbe
-        apply ExpClass.def.mpr
+        have soundness' := @soundness
+        translate `convr `convr_Setoid
+        hide soundness'
         -- f1 ~ f2 ~ nbe f2 = nbe f1
         -- "rewrite [f1_r_f2, f2_r_nbe, ← soundness f1_r_f2]"
-        rw [f1_r_f2, f2_r_nbe, ← soundness $ ExpClass.def.mpr f1_r_f2]
+        rw [f1_r_f2, f2_r_nbe, ← soundness' f1_r_f2]
       · intro e' Re'
         rewrite [βIH (f1 ⬝ e') (f2 ⬝ e') (f1_r_f2.app convr.refl)]
         rcases R_f2 with ⟨_, h0⟩
         exact h0 e' Re'
 
-
-def numeral : ℕ → Exp Ty.Nat
-| 0 => zero
-
-| n+1 => succ ⬝ (numeral n)
-
-lemma reify_Nat : ∃ n, reify Ty.Nat k = (numeral n) :=
-  by
-  induction k
-  case zero =>
-    use 0; rfl
-
-  case succ k' IH =>
-    rcases IH with ⟨n, eq⟩
-    use n+1
-    calc
-      reify Ty.Nat k'.succ = succ ⬝ (reify Ty.Nat k') := rfl
-      _ = succ ⬝ (numeral n) := by rw [eq]
-      _ = numeral (n+1)      := rfl
-
-lemma nbe_Nat : ∃ n, nbe Ty.Nat e = numeral n := reify_Nat
 
 lemma R_numeral : R Ty.Nat (numeral n) :=
   by
@@ -247,11 +190,12 @@ lemma R_numeral : R Ty.Nat (numeral n) :=
     unfold numeral
     have eq : nbe Ty.Nat (succ ⬝ numeral n') = succ ⬝ (nbe Ty.Nat $ numeral n') := rfl
     -- Translate "convr a b" to "⟦a⟧ = ⟦b⟧":
-    replace IH := ExpClass.def.mp IH
-    apply ExpClass.def.mpr
+    have convr.app' := @convr.app
+    translate `convr `convr_Setoid
+    hide convr.app'
     -- succ ⬝ numeral n' ~ succ ⬝ nbe (numeral n') = nbe (succ ⬝ numeral n')
     -- "rewrite [IH, eq]"
-    rw [ExpClass.app_arg IH, eq]
+    rw [convr.app' rfl IH, eq]
 
 -- for all e, R a e
 lemma all_R {e : Exp a} : R a e :=
@@ -266,13 +210,14 @@ lemma all_R {e : Exp a} : R a e :=
       · have e'_r_nbe := R_convr_nbe Re'; clear Re'
         have eq : nbe (b ⇒' a) (K ⬝ e') = K ⬝ nbe a e' := rfl
         -- Translate "convr a b" to "⟦a⟧ = ⟦b⟧"
-        replace e'_r_nbe := ExpClass.def.mp e'_r_nbe
-        apply ExpClass.def.mpr
+        have convr.app' := @convr.app
+        translate `convr `convr_Setoid
+        hide convr.app'
         -- K ⬝ e' ~ K ⬝ nbe e' = nbe (K ⬝ e')
         -- "rewrite [e'_r_nbe, eq]"
-        rw [ExpClass.app_arg e'_r_nbe, eq]
+        rw [convr.app' rfl e'_r_nbe, eq]
 
-      · intro e'' _
+      · intro e'' Re''; clear Re''
         --convr-rewriting here
         -- R (K ⬝ e' ⬝ e'') = R e'
         -- "rewrite [convr.K]"
@@ -287,28 +232,30 @@ lemma all_R {e : Exp a} : R a e :=
       · have x_r_nbe := R_convr_nbe Rx; clear Rx
         have eq : nbe ((a ⇒' b) ⇒' a ⇒' c) (S ⬝ x) = S ⬝ nbe (a ⇒' b ⇒' c)  x := rfl
         -- Translate "convr a b" to "⟦a⟧ = ⟦b⟧"
-        replace x_r_nbe := ExpClass.def.mp x_r_nbe
-        apply ExpClass.def.mpr
+        have convr.app' := @convr.app
+        translate `convr `convr_Setoid
+        hide convr.app'
         -- S ⬝ x ~ S ⬝ nbe x = nbe (S ⬝ x)
         -- "rewrite [x_r_nbe, eq]"
-        rw [ExpClass.app_arg x_r_nbe, eq]
+        rw [convr.app' rfl x_r_nbe, eq]
       · intro y Ry
         apply And.intro
         · have x_r_nbe := R_convr_nbe Rx; clear Rx; have y_r_nbe := R_convr_nbe Ry; clear Ry
           have eq : nbe (a ⇒' c) (S ⬝ x ⬝ y) = S ⬝ nbe (a ⇒' b ⇒' c) x ⬝ nbe (a ⇒' b) y := rfl
           -- Translate "convr a b" to "⟦a⟧ = ⟦b⟧"
-          replace x_r_nbe := ExpClass.def.mp x_r_nbe; replace y_r_nbe := ExpClass.def.mp y_r_nbe
-          apply ExpClass.def.mpr
+          have convr.app' := @convr.app
+          translate `convr `convr_Setoid
+          hide convr.app'
           -- S ⬝ x ⬝ y ~ S ⬝ nbe x ⬝ y ~ S ⬝ nbe x ⬝ nbe y = nbe (S ⬝ x ⬝ y)
           -- "rewrite [x_r_nbe, y_r_nbe, eq]"
-          rw [ExpClass.app_fun $ ExpClass.app_arg x_r_nbe, ExpClass.app_arg y_r_nbe, eq]
+          rw [convr.app' (convr.app' rfl x_r_nbe) rfl, convr.app' rfl y_r_nbe, eq]
         · intro z Rz
           -- convr-rewriting here
           -- "rewrite [convr.S]"
           rewrite [convr_R_iff (S ⬝ x ⬝ y ⬝ z) _ convr.S]
-          rcases Rx with ⟨_, Rxz⟩; specialize Rxz z Rz
-          rcases Ry with ⟨_, Ryz⟩; specialize Ryz z Rz
-          rcases Rxz with ⟨_, Rxzyz⟩; specialize Rxzyz (y ⬝ z) Ryz
+          rcases Rx with ⟨left, Rxz⟩; clear left; specialize Rxz z Rz
+          rcases Ry with ⟨left, Ryz⟩; clear left; specialize Ryz z Rz
+          rcases Rxz with ⟨left, Rxzyz⟩; clear left; specialize Rxzyz (y ⬝ z) Ryz
           exact Rxzyz
 
   case App α β f x Rf Rx =>
@@ -325,11 +272,12 @@ lemma all_R {e : Exp a} : R a e :=
       unfold R at *; rename' Rx => x_r_nbe
       have eq : nbe Ty.Nat (succ ⬝ x) = succ ⬝ (nbe Ty.Nat x) := rfl
       -- Translate "convr a b" to "⟦a⟧ = ⟦b⟧"
-      replace x_r_nbe := ExpClass.def.mp x_r_nbe
-      apply ExpClass.def.mpr
+      have convr.app' := @convr.app
+      translate `convr `convr_Setoid
+      hide convr.app'
       -- succ ⬝ x ~ succ ⬝ nbe x = nbe (succ ⬝ x)
       -- "rewrite [x_r_nbe, eq]"
-      rw [ExpClass.app_arg x_r_nbe, eq]
+      rw [convr.app' rfl x_r_nbe, eq]
 
   case recN α =>
     apply And.intro
@@ -339,42 +287,39 @@ lemma all_R {e : Exp a} : R a e :=
       · have e'_r_nbe := R_convr_nbe Re'; clear Re'
         have eq : nbe ((Ty.Nat ⇒' α ⇒' α) ⇒' Ty.Nat ⇒' α) (recN ⬝ e') = recN ⬝ nbe α e' := rfl
         -- Translate "convr a b" to "⟦a⟧ = ⟦b⟧"
-        replace e'_r_nbe := ExpClass.def.mp e'_r_nbe
-        apply ExpClass.def.mpr
+        have convr.app' := @convr.app
+        translate `convr `convr_Setoid
+        hide convr.app'
         -- recN ⬝ e' ~ recN ⬝ nbe e' = nbe (recN ⬝ e')
         -- "rewrite [e'_r_nbe, eq]"
-        rw [ExpClass.app_arg e'_r_nbe, eq]
+        rw [convr.app' rfl e'_r_nbe, eq]
       · intro e'' Re''
         apply And.intro
         · have e'_r_nbe := R_convr_nbe Re'; clear Re'; have e''_r_nbe := R_convr_nbe Re''; clear Re''
           have eq : nbe (Ty.Nat ⇒' α) (recN ⬝ e' ⬝ e'') = recN ⬝ nbe α e' ⬝ nbe (Ty.Nat ⇒' α ⇒' α) e'' := rfl
           -- Translate "convr a b" to "⟦a⟧ = ⟦b⟧"
-          replace e'_r_nbe := ExpClass.def.mp e'_r_nbe; replace e''_r_nbe := ExpClass.def.mp e''_r_nbe
-          apply ExpClass.def.mpr
+          have convr.app' := @convr.app
+          translate `convr `convr_Setoid
+          hide convr.app'
           -- recN ⬝ e' ⬝ e'' ~ recN ⬝ nbe e' ⬝ e'' ~ recN ⬝ nbe e' ⬝ nbe e'' = nbe (recN ⬝ e' ⬝ e'')
           -- "rewrite [e'_r_nbe, e''_r_nbe, eq]"
-          rw [ExpClass.app_fun $ ExpClass.app_arg e'_r_nbe, ExpClass.app_arg e''_r_nbe, eq]
+          rw [convr.app' (convr.app' rfl e'_r_nbe) rfl, convr.app' rfl e''_r_nbe, eq]
         · intro n Rn
           have n_r_nbe := Rn; unfold R at n_r_nbe
           -- "rewrite [n_r_nbe]"
           rewrite [convr_R_iff (recN ⬝ e' ⬝ e'' ⬝ n) (recN ⬝ e' ⬝ e'' ⬝ (nbe Ty.Nat n)) (convr.refl.app n_r_nbe)]
-          have eq : ∃ n₁, nbe Ty.Nat n = numeral n₁ := nbe_Nat
-          rcases eq with ⟨n₁, eq⟩; rewrite [eq] at n_r_nbe ⊢; clear eq
-          (have R_numeral_n₁ : R Ty.Nat (numeral n₁) := by exact (convr_R_iff n (numeral n₁) n_r_nbe).mp Rn); clear Rn n_r_nbe n
-          induction n₁
+          unfold nbe; simp [reify]
+          induction ((Exp_inter Ty.Nat n))
           · unfold numeral
             -- "rewrite [convr.recN_zero]"
             exact (convr_R_iff (recN ⬝ e' ⬝ e'' ⬝ zero) e' convr.recN_zero).mpr Re'
           · rename_i n' IH
-            unfold numeral at R_numeral_n₁ ⊢
-            -- "rewrite [convr.recN_succ]"
-            rewrite [convr_R_iff (recN ⬝ e' ⬝ e'' ⬝ (succ ⬝ numeral n')) (e'' ⬝ (numeral n') ⬝ (recN ⬝ e' ⬝ e'' ⬝ (numeral n'))) convr.recN_succ]
-            have R_numeral_n' : R Ty.Nat (numeral n') := R_numeral
-            specialize IH R_numeral_n'
-            rcases Re'' with ⟨_, h0⟩
+            apply (convr_R_iff (.recN ⬝ e' ⬝ e'' ⬝ (.succ ⬝ numeral n')) (e'' ⬝ (numeral n') ⬝ (.recN ⬝ e' ⬝ e'' ⬝ (numeral n'))) convr.recN_succ).mpr
+            have R_numeral_n' : R Ty.Nat (numeral n') := by exact R_numeral
+            rcases Re'' with ⟨left, h0⟩; clear left
             specialize h0 (numeral n') R_numeral_n'
-            rcases h0 with ⟨_, h0⟩
-            exact h0 (recN ⬝ e' ⬝ e'' ⬝ numeral n') IH
+            rcases h0 with ⟨left, h0⟩; clear left
+            exact h0 (.recN ⬝ e' ⬝ e'' ⬝ numeral n') IH
 
 
 -- e ~ nbe a e
@@ -385,10 +330,12 @@ lemma completeness : nbe a e = nbe a e' → convr e e' :=
   by
   intro eq
   -- Translate "convr a b" to "⟦a⟧ = ⟦b⟧"
-  apply ExpClass.def.mpr
+  have convr_nbe' := @convr_nbe
+  translate `convr `convr_Setoid
+  hide convr_nbe'
   -- e ~ nbe e = nbe e' ~ e'
   -- "rewrite [convr_nbe, eq, ← convr_nbe]"
-  rw [ExpClass.def.mp convr_nbe, eq, ← ExpClass.def.mp convr_nbe]
+  rw [convr_nbe', eq, ← convr_nbe']
 
 -- e ~ e' ↔ nbe a e = nbe a e'
 lemma correctness {e e' : Exp a} : convr e e' ↔ nbe a e = nbe a e' := ⟨soundness, completeness⟩
