Tactic/setoidRw.lean
@@ -3,10 +3,236 @@ import Mathlib.Tactic
 
 open Lean Elab Tactic Term Meta
 
---set_option pp.universes true
+/-Prints out the current Environment.
+-/
+def printEnv : CoreM Unit := do
+  let env ← getEnv
+  for (name, info)
+    in (env.constants).toList.take 150 do
+        let type := info.type
+        logInfo s!"{name} : {type}"
+elab "printEnv" : tactic => do printEnv
 
--- From: https://cs.ioc.ee/ewscs/2009/dybjer/mainPalmse-revised.pdf
+/-Prints out the current Local-Context
+-/
+def printLocalCtxt : TacticM Unit :=
+  withMainContext do
+    let goal ← getMainGoal
+    let localCtxt ← getLCtx
+    for localDecl in localCtxt do
+        let expr := localDecl.toExpr
+        let name := localDecl.userName
+        let type := localDecl.type
+        logInfo s!"{name} := {expr}"
+        logInfo s!": {type}"
+        logInfo " "
+    logInfo " "
+    logInfo s!"goal"
+    logInfo s!": {←goal.getType}"
+elab "printLocalCtxt" : tactic => do printLocalCtxt
 
+/--
+  `hide h` removes the given hypotheses from the *pretty-printed*
+  goal state, but they remain usable by name in the proof.
+-/
+elab "hide " n:ident : tactic => do
+  withMainContext do
+    let n         := (n.getId)
+    let goal      := ← getMainGoal
+    let localCtxt := ← getLCtx
+    let some fvar := localCtxt.findFromUserName? n | throwError s!"{n} is not in Local-Context!"
+    goal.setFVarKind (fvar.fvarId) (LocalDeclKind.implDetail)
+
+
+-- Example usage
+example (p q r : Prop) (h : p → q) (h' : q → r) (hp : p) : r := by
+  /- Goal state initially:
+  p q r : Prop
+  h : p → q
+  h' : q → r
+  hp : p
+  ⊢ r
+  -/
+  hide hp
+  /- After `hide hp`, goal state:
+  p q r : Prop
+  h : p → q
+  h' : q → r
+  ⊢ r
+  -/
+  exact h' (h hp)
+
+
+/-
+Our Grammar for Inductive setoids is:
+  inductive R : (x₁ : T₁) → (x₂ : T₂) → ⋯ → (xₙ : Tₙ) → (_ : X) → (_ : X) → Prop
+    where
+    · (x₁ : T₁) → (x₂ : T₂) → ⋯ → (xₙ : Tₙ) → (_ : X) → (_ : X) → Prop  is a telescope
+    · X is our carrier-set
+
+  instance R_Setoid : (x₁ : T₁) → (x₂ : T₂) → ⋯ → (xₙ : Tₙ) → Setoid X
+                 := λ (x₁ : T₁) (x₂ : T₂) ⋯ (xₙ : Tₙ) => ⟨r := R, iseqv := ⋯⟩
+-/
+/-
+grammar ⟨r := R, iseqv := ⋯⟩  := ⟨X⟩
+-/
+
+
+-- R : (x₁ : T₁) → (x₂ : T₂) → ⋯ → (xₙ : Tₙ) → (_ : X) → (_ : X) → Prop
+-- destruct R := ⟨[(x₁ : T₁), ⋯, (xₙ : Tₙ)], (_ : X) → (_ : X) → Prop⟩
+def destructR (R : Name) : MetaM (Array Expr × Expr) := do
+  let R := .const R []
+  let RType := ← inferType R
+  let n_plus_two := RType.getNumHeadForalls
+  forallBoundedTelescope RType (some $ n_plus_two-2) fun xs X_X_Prop => do
+    logInfo s!"{← mkForallFVars xs X_X_Prop}"
+    return ⟨xs, X_X_Prop⟩
+
+
+-- R        : (x₁ : T₁) → (x₂ : T₂) → ⋯ → (xₙ : Tₙ) → (_ : X) → (_ : X) → Prop
+-- R_Setoid : (x₁ : T₁) → (x₂ : T₂) → ⋯ → (xₙ : Tₙ) → Setoid X
+
+-- QuotientExpr R R_Setoid := (x₁ : T₁) → (x₂ : T₂) → ⋯ → (xₙ : Tₙ) → Quotient X (R_Setoid x₁ ⋯ xₙ)
+def QuotientExpr (R : Name) (R_Setoid : Name) : MetaM Expr := do
+  let R_Setoid  := (Expr.const R_Setoid [])
+
+  let R := .const R []
+  let RType := ← inferType R
+  let n_plus_two := RType.getNumHeadForalls
+  forallBoundedTelescope RType (some $ n_plus_two-2) fun xs X_X_Prop => do
+    let X := X_X_Prop.bindingDomain!
+    let Quotient := (← mkAppOptM ``Quotient $ #[some X] ++ #[some $ mkAppN (R_Setoid) xs ])
+    mkLambdaFVars xs Quotient
+
+
+-- R        : (x₁ : T₁) → (x₂ : T₂) → ⋯ → (xₙ : Tₙ) → (_ : X) → (_ : X) → Prop
+-- R_Setoid : (x₁ : T₁) → (x₂ : T₂) → ⋯ → (xₙ : Tₙ) → Setoid X
+
+-- mkQuotientEq R R_Setoid := λ x₁ ⋯ xₙ e1 e2 => ⟦e1⟧ = ⟦e2⟧
+def mkQuotientEq (R : Name) (R_Setoid : Name) : MetaM Expr := do
+  let R_Setoid  := (Expr.const R_Setoid [])
+
+
+  let R := .const R []
+  let RType := ← inferType R
+  let n_plus_two := RType.getNumHeadForalls
+  forallBoundedTelescope RType (some $ n_plus_two) fun xs_e1_e2 _Prop => do
+    let xs := xs_e1_e2.pop.pop
+    let e1 := xs_e1_e2.pop.toList.getLast!
+    let e2 := xs_e1_e2.toList.getLast!
+    let X := ← inferType e2
+    let bb_e1_dd := (← mkAppOptM ``Quotient.mk $ #[some X] ++ #[some $ mkAppN (R_Setoid) xs, e1])
+    let bb_e2_dd := (← mkAppOptM ``Quotient.mk $ #[some X] ++ #[some $ mkAppN (R_Setoid) xs, e2])
+    let eq := ← mkEq bb_e1_dd bb_e2_dd
+    mkLambdaFVars xs_e1_e2 eq
+
+
+-- R        : (x₁ : T₁) → (x₂ : T₂) → ⋯ → (xₙ : Tₙ) → (_ : X) → (_ : X) → Prop
+-- R_Setoid : (x₁ : T₁) → (x₂ : T₂) → ⋯ → (xₙ : Tₙ) → Setoid X
+
+-- mkR_Eq_Quotient R R_Setoid := R = λ x₁ ⋯ xₙ e1 e2 => ⟦e1⟧ = ⟦e2⟧
+def mkR_Eq_Quotient (R : Name) (R_Setoid : Name) : MetaM Expr := do
+  let QuotientEq := ← mkQuotientEq R R_Setoid
+  let R := .const R []
+  mkEq R QuotientEq
+
+
+-- R        : (x₁ : T₁) → (x₂ : T₂) → ⋯ → (xₙ : Tₙ) → (_ : X) → (_ : X) → Prop
+-- R_Setoid : (x₁ : T₁) → (x₂ : T₂) → ⋯ → (xₙ : Tₙ) → Setoid X
+
+-- Adds "R_eq : R = λ x₁ ⋯ xₙ e1 e2 => ⟦e1⟧ = ⟦e2⟧" to the environment
+def addR_eq (R : Name) (R_Setoid : Name) : TermElabM Unit := do
+  -- Build the type "R = λ x₁ ⋯ xₙ e1 e2 => ⟦e1⟧ = ⟦e2⟧"
+  let type := ← mkR_Eq_Quotient R R_Setoid
+
+  -- Elaborate automated tactic proof as an expression
+  -- Ensuring there are no meta-variables (so kernel doesn't complain)
+  let pf := ← elabTerm (← `(by
+      funext
+      apply propext
+      apply Iff.intro
+      exact λ h => Quotient.sound h
+      exact λ h => Quotient.exact h
+    )) (some type)
+  Term.synthesizeSyntheticMVarsNoPostponing
+  let pf ← instantiateMVars pf
+
+  -- Add "R_eq : R = λ x₁ ⋯ xₙ e1 e2 => ⟦e1⟧ = ⟦e2⟧" to the environment
+  let env              := ← getEnv
+  let restrictedPrefix := env.asyncPrefix?.casesOn' ("") (λ name => name.toString ++ ".")
+  let decl := Declaration.thmDecl {
+    name        := (restrictedPrefix ++ R.toString ++ "_eq").toName
+    levelParams := []
+    type        := type
+    value       := pf
+  }
+  addDecl decl
+  compileDecl decl
+elab "addR_eq" R:name R_Setoid:name : tactic => do addR_eq R.getName R_Setoid.getName
+
+
+-- R        : (x₁ : T₁) → (x₂ : T₂) → ⋯ → (xₙ : Tₙ) → (_ : X) → (_ : X) → Prop
+-- R_Setoid : (x₁ : T₁) → (x₂ : T₂) → ⋯ → (xₙ : Tₙ) → Setoid X
+def translate (R : Name) (R_Setoid : Name) : TacticM Unit :=
+  withMainContext do
+    -- Add "R_eq : R = λ x₁ ⋯ xₙ e1 e2 => ⟦e1⟧ = ⟦e2⟧" to the environment
+    let env       := ← getEnv
+    let restrictedPrefix := env.asyncPrefix?.casesOn' ("") (λ name => name.toString ++ ".")
+    let R_eq      := (restrictedPrefix ++ R.toString ++ "_eq").toName
+    if ! env.contains R_eq
+    then
+      addR_eq R R_Setoid
+
+    -- Revert all localHyps (last-to-first localHyps)
+    let localHyps := (← getLocalHyps).map (λ expr => (expr.fvarId!))
+    let goal      := ← getMainGoal
+    let (_, goal) := ← goal.revert (preserveOrder := True) (localHyps)
+    replaceMainGoal [goal]
+
+    -- Generalize on R
+    let R_Ident    := mkIdent R
+    let R'_Ident   := mkIdent (R.toString ++ "'").toName
+    let eq_Ident  := mkIdent ("eq").toName
+    evalTactic (← `(tactic | generalize $eq_Ident:ident : (@$R_Ident:ident) = $R'_Ident:ident))
+
+    -- Rewrite "R_eq : R = R_eq : R = (λ x₁ ⋯ xₙ e1 e2 => ⟦e1⟧ = ⟦e2⟧)"
+    -- at "eq : R = R'"
+    let R_eq_Ident := mkIdent R_eq
+    evalTactic (← `(tactic | rewrite [($R_eq_Ident:ident)] at ($eq_Ident:ident)))
+
+    -- Substitute "eq : (λ x₁ ⋯ xₙ e1 e2 => ⟦e1⟧ = ⟦e2⟧)  =  R'" everywhere
+    evalTactic (← `(tactic | subst ($eq_Ident:ident)))
+
+    -- Beta-reduce the goal
+    evalTactic (← `(tactic | beta_reduce))
+
+    -- Re-intro all our localHyps (first-to-last localHyps)
+    let goal      := ← getMainGoal
+    let localHyps := (← localHyps.mapM (λ fvar => fvar.getUserName)).toList
+    let n := localHyps.length
+    let (_, goal) := ← goal.introN n (givenNames := localHyps)
+    replaceMainGoal [goal]
+elab "translate" R:name R_Setoid:name : tactic => do translate @R.getName @R_Setoid.getName
+/-
+Step 1: Revert EVERYTHING to get a single Target with an empty LocalCtxt
+
+Step 2: Translate Target
+
+Step 3: Intro EVERYTHING with all their original names
+
+This avoids breaking anything due to dependent products.
+This way we guarantee translating all "R"s in one single step.
+-/
+
+
+
+
+
+
+
+
+
+/-
 inductive Ty : Type
 | Nat : Ty
 | arrow : Ty → Ty → Ty
@@ -53,224 +279,25 @@ instance convr_Setoid : Setoid (Exp α) :=
 
 def ExpClass α := Quotient (@convr_Setoid α)
 
-/-
-lemma convr_eq :
-  (@convr) = (λ α => λ (e1 e2 : Exp α) => ((⟦e1⟧ : ExpClass α) = ⟦e2⟧)) :=
-  by
-  show_term
-    funext
-    apply propext
-    apply Iff.intro
-    exact λ h => Quotient.sound h
-    exact λ h => Quotient.exact h
--/
-
-/-Prints out the current Environment.
--/
-def printEnv : CoreM Unit := do
-  let env ← getEnv
-  for (name, info)
-    in (env.constants).toList.take 150 do
-        let type := info.type
-        logInfo s!"{name} : {type}"
-elab "printEnv" : tactic => do printEnv
-
-/-Prints out the current Local-Context
--/
-def printLocalCtxt : TacticM Unit :=
-  withMainContext do
-    let goal ← getMainGoal
-    let localCtxt ← getLCtx
-    for localDecl in localCtxt do
-        let expr := localDecl.toExpr
-        let name := localDecl.userName
-        let type := localDecl.type
-        logInfo s!"{name} := {expr}"
-        logInfo s!": {type}"
-        logInfo " "
-    logInfo " "
-    logInfo s!"goal"
-    logInfo s!": {←goal.getType}"
-elab "printLocalCtxt" : tactic => do printLocalCtxt
-
-
-/-
-Our Grammar for Inductive setoids is:
-  inductive R : (x₁ : T₁) → (x₂ : T₂) → ⋯ → (xₙ : Tₙ) → (_ : X) → (_ : X) → Prop
-    where
-    · (x₁ : T₁) → (x₂ : T₂) → ⋯ → (xₙ : Tₙ) → (_ : X) → (_ : X) → Prop  is a telescope
-    · X is our carrier-set
-
-  instance R_Setoid : (x₁ : T₁) → (x₂ : T₂) → ⋯ → (xₙ : Tₙ) → Setoid X
-                 := λ (x₁ : T₁) (x₂ : T₂) ⋯ (xₙ : Tₙ) => ⟨r := R, iseqv := ⋯⟩
--/
-/-
-grammar ⟨r := R, iseqv := ⋯⟩  := ⟨X⟩
--/
-
-
--- R : (x₁ : T₁) → (x₂ : T₂) → ⋯ → (xₙ : Tₙ) → (_ : X) → (_ : X) → Prop
--- destruct R := ⟨[(x₁ : T₁), ⋯, (xₙ : Tₙ)], (_ : X) → (_ : X) → Prop⟩
-def destructR (R : Name) : MetaM (Array Expr × Expr) := do
-  let R := .const R []
-  let RType := ← inferType R
-  let n_plus_two := RType.getNumHeadForalls
-  forallBoundedTelescope RType (some $ n_plus_two-2) fun xs X_X_Prop => do
-    logInfo s!"{← mkForallFVars xs X_X_Prop}"
-    return ⟨xs, X_X_Prop⟩
+-- destructR
 #eval destructR ``convr
-
-
--- R        : (x₁ : T₁) → (x₂ : T₂) → ⋯ → (xₙ : Tₙ) → (_ : X) → (_ : X) → Prop
--- R_Setoid : (x₁ : T₁) → (x₂ : T₂) → ⋯ → (xₙ : Tₙ) → Setoid X
-
--- QuotientExpr R R_Setoid := (x₁ : T₁) → (x₂ : T₂) → ⋯ → (xₙ : Tₙ) → Quotient X (R_Setoid x₁ ⋯ xₙ)
-def QuotientExpr (R : Name) (R_Setoid : Name) : MetaM Expr := do
-  let R_Setoid  := (Expr.const R_Setoid [])
-
-  let R := .const R []
-  let RType := ← inferType R
-  let n_plus_two := RType.getNumHeadForalls
-  forallBoundedTelescope RType (some $ n_plus_two-2) fun xs X_X_Prop => do
-    let X := X_X_Prop.bindingDomain!
-    let Quotient := (← mkAppOptM ``Quotient $ #[some X] ++ #[some $ mkAppN (R_Setoid) xs ])
-    mkLambdaFVars xs Quotient
+-- QuotientExpr
 #eval do check $ ← QuotientExpr `convr `convr_Setoid
 #eval do ppExpr $ ← QuotientExpr `convr `convr_Setoid
 #eval QuotientExpr `convr `convr_Setoid
 #check fun α => @Quotient (Exp α) (@convr_Setoid α)
-
-
--- R        : (x₁ : T₁) → (x₂ : T₂) → ⋯ → (xₙ : Tₙ) → (_ : X) → (_ : X) → Prop
--- R_Setoid : (x₁ : T₁) → (x₂ : T₂) → ⋯ → (xₙ : Tₙ) → Setoid X
-
--- mkQuotientEq R R_Setoid := λ x₁ ⋯ xₙ e1 e2 => ⟦e1⟧ = ⟦e2⟧
-def mkQuotientEq (R : Name) (R_Setoid : Name) : MetaM Expr := do
-  let R_Setoid  := (Expr.const R_Setoid [])
-
-
-  let R := .const R []
-  let RType := ← inferType R
-  let n_plus_two := RType.getNumHeadForalls
-  forallBoundedTelescope RType (some $ n_plus_two) fun xs_e1_e2 _Prop => do
-    let xs := xs_e1_e2.pop.pop
-    let e1 := xs_e1_e2.pop.toList.getLast!
-    let e2 := xs_e1_e2.toList.getLast!
-    let X := ← inferType e2
-    let bb_e1_dd := (← mkAppOptM ``Quotient.mk $ #[some X] ++ #[some $ mkAppN (R_Setoid) xs, e1])
-    let bb_e2_dd := (← mkAppOptM ``Quotient.mk $ #[some X] ++ #[some $ mkAppN (R_Setoid) xs, e2])
-    let eq := ← mkEq bb_e1_dd bb_e2_dd
-    mkLambdaFVars xs_e1_e2 eq
+-- mkQuotientEq
 #eval do check $ ← mkQuotientEq `convr `convr_Setoid
 #eval do ppExpr $ ← mkQuotientEq `convr `convr_Setoid
 #eval mkQuotientEq `convr `convr_Setoid
 #check fun α e1 e2 => (@Quotient.mk (Exp α) (@convr_Setoid α) e1) = (@Quotient.mk (Exp α) (@convr_Setoid α) e2)
-
--- R        : (x₁ : T₁) → (x₂ : T₂) → ⋯ → (xₙ : Tₙ) → (_ : X) → (_ : X) → Prop
--- R_Setoid : (x₁ : T₁) → (x₂ : T₂) → ⋯ → (xₙ : Tₙ) → Setoid X
-
--- mkR_Eq_Quotient R R_Setoid := R = λ x₁ ⋯ xₙ e1 e2 => ⟦e1⟧ = ⟦e2⟧
-def mkR_Eq_Quotient (R : Name) (R_Setoid : Name) : MetaM Expr := do
-  let QuotientEq := ← mkQuotientEq R R_Setoid
-  let R := .const R []
-  mkEq R QuotientEq
+-- mkR_Eq_Quotient
 #eval do check $ ← mkR_Eq_Quotient `convr `convr_Setoid
 #eval do ppExpr $ ← mkR_Eq_Quotient `convr `convr_Setoid
 #eval mkR_Eq_Quotient ``convr ``convr_Setoid
 #check @convr = fun {α} e1 e2 ↦ ⟦e1⟧ = ⟦e2⟧
 
 
--- R        : (x₁ : T₁) → (x₂ : T₂) → ⋯ → (xₙ : Tₙ) → (_ : X) → (_ : X) → Prop
--- R_Setoid : (x₁ : T₁) → (x₂ : T₂) → ⋯ → (xₙ : Tₙ) → Setoid X
-
--- Adds "R_eq : R = λ x₁ ⋯ xₙ e1 e2 => ⟦e1⟧ = ⟦e2⟧" to the environment
-def addR_eq (R : Name) (R_Setoid : Name) : TermElabM Unit := do
-  -- Build the type "R = λ x₁ ⋯ xₙ e1 e2 => ⟦e1⟧ = ⟦e2⟧"
-  let type := ← mkR_Eq_Quotient R R_Setoid
-
-  -- Elaborate automated tactic proof as an expression
-  -- Ensuring there are no meta-variables (so kernel doesn't complain)
-  let pf := ← elabTerm (← `(by
-      funext
-      apply propext
-      apply Iff.intro
-      exact λ h => Quotient.sound h
-      exact λ h => Quotient.exact h
-    )) (some type)
-  Term.synthesizeSyntheticMVarsNoPostponing
-  let pf ← instantiateMVars pf
-
-  -- Add "R_eq : R = λ x₁ ⋯ xₙ e1 e2 => ⟦e1⟧ = ⟦e2⟧" to the environment
-  let env              := ← getEnv
-  let restrictedPrefix := env.asyncPrefix?.casesOn' ("") (λ name => name.toString ++ ".")
-  let decl := Declaration.thmDecl {
-    name        := (restrictedPrefix ++ R.toString ++ "_eq").toName
-    levelParams := []
-    type        := type
-    value       := pf
-  }
-  addDecl decl
-  compileDecl decl
-
-
-
-elab "addR_eq" R:name R_Setoid:name : tactic => do addR_eq R.getName R_Setoid.getName
-
-
--- R        : (x₁ : T₁) → (x₂ : T₂) → ⋯ → (xₙ : Tₙ) → (_ : X) → (_ : X) → Prop
--- R_Setoid : (x₁ : T₁) → (x₂ : T₂) → ⋯ → (xₙ : Tₙ) → Setoid X
-def translate (R : Name) (R_Setoid : Name) : TacticM Unit :=
-  withMainContext do
-    -- Add "R_eq : R = λ x₁ ⋯ xₙ e1 e2 => ⟦e1⟧ = ⟦e2⟧" to the environment
-    let env       := ← getEnv
-    let restrictedPrefix := env.asyncPrefix?.casesOn' ("") (λ name => name.toString ++ ".")
-    let R_eq      := (restrictedPrefix ++ R.toString ++ "_eq").toName
-    if ! env.contains R_eq
-    then
-      addR_eq R R_Setoid
-
-    -- Revert all localHyps (last-to-first localHyps)
-    let localHyps := (← getLocalHyps).map (λ expr => (expr.fvarId!))
-    let goal      := ← getMainGoal
-    let (_, goal) := ← goal.revert (preserveOrder := True) (localHyps)
-    replaceMainGoal [goal]
-
-    -- Generalize on R
-    let R_Ident    := mkIdent R
-    let R'_Ident   := mkIdent (R.toString ++ "'").toName
-    let eq_Ident  := mkIdent ("eq").toName
-    evalTactic (← `(tactic | generalize $eq_Ident:ident : (@$R_Ident:ident) = $R'_Ident:ident))
-
-    -- Rewrite "R_eq : R = R_eq : R = (λ x₁ ⋯ xₙ e1 e2 => ⟦e1⟧ = ⟦e2⟧)"
-    -- at "eq : R = R'"
-    let R_eq_Ident := mkIdent R_eq
-    evalTactic (← `(tactic | rewrite [($R_eq_Ident:ident)] at ($eq_Ident:ident)))
-
-    -- Substitute "eq : (λ x₁ ⋯ xₙ e1 e2 => ⟦e1⟧ = ⟦e2⟧)  =  R'" everywhere
-    evalTactic (← `(tactic | subst ($eq_Ident:ident)))
-
-    -- Beta-reduce the goal
-    evalTactic (← `(tactic | beta_reduce))
-
-    -- Re-intro all our localHyps (first-to-last localHyps)
-    let goal      := ← getMainGoal
-    let localHyps := (← localHyps.mapM (λ fvar => fvar.getUserName)).toList
-    let n := localHyps.length
-    let (_, goal) := ← goal.introN n (givenNames := localHyps)
-    replaceMainGoal [goal]
-
-elab "translate" R:name R_Setoid:name : tactic => do translate @R.getName @R_Setoid.getName
-
-/-
-Step 1: Revert EVERYTHING to get a single Target with an empty LocalCtxt
-
-Step 2: Translate Target
-
-Step 3: Intro EVERYTHING with all their original names
-
-This avoids breaking anything due to dependent products.
-This way we guarantee translating all "R"s in one single step.
--/
 example {α : Ty} {a b : Exp α}
                         (f : (x y : Exp α) → (@convr α x y) → Nat)
                         (hf : (x y : Exp α) → (xRy : @convr α x y) → f x y xRy = 3)
@@ -327,7 +354,7 @@ example : (⟦a⟧ : ExpClass (β ⇒' α)) = ⟦b⟧ → (⟦c⟧ : ExpClass β
 
 
 
-
+/-
 -- Alternate implementation idea: Have a custom typeclass "SetoidRewrite"
 -- that extends "Setoid R" has an addtional "rEq" field.
 -- This would also automatically add our equality lemma "R_eq" to the environment.
@@ -348,34 +375,7 @@ instance {α_Setoid : Setoid α} : SetoidRewrite α :=
       exact fun a ↦ Quotient.sound a
       exact fun a ↦ Quotient.exact a
                                     }
-
-
-lemma ExpClass_test :
-  (λ α => @convr α) = (λ α => λ (e1 e2 : Exp α) => ((⟦e1⟧ : ExpClass α) = ⟦e2⟧)) :=
-  by
-
-  have rEq' := λ α => @SetoidRewrite.rEq (Exp α)
-  show_term
-    apply funext; intro α
-    apply funext ; intro e1
-    apply funext ; intro e2
-    apply propext
-    apply Iff.intro
-    exact fun a => Quotient.sound a
-    exact fun a => Quotient.exact a
-
-lemma ExpClass_test2 {α} {e1 e2 : Exp α} :
-  (@convr α e1 e2) = (((⟦e1⟧ : ExpClass α) = ⟦e2⟧)) :=
-  by
-  show_term
-    apply propext
-    apply Iff.intro
-    exact fun a => Quotient.sound a
-    exact fun a => Quotient.exact a
-
-
-def Eq' : {α : Ty} → (Exp α) → (Exp α) → Prop := λ {α : Ty} (e1 e2 : Exp α) => ((⟦e1⟧ : ExpClass α) = ⟦e2⟧)
-
+-/
 
 lemma ExpClass_K {α : Ty} {β : Ty} {x : Exp α} (y : Exp β) : (⟦K ⬝ x ⬝ y⟧ : ExpClass α) = ⟦x⟧ :=
   by
@@ -490,7 +490,7 @@ by
 def R : (a : Ty) → (e : Exp a) → Prop
 | Ty.Nat, e       => convr e (nbe Ty.Nat e)
 
-| Ty.arrow α β, e => convr e (nbe (α ⇒' β) e)  ∧  ∀ e', R α e' → R β (App e e')
+| Ty.arrow α β, e => convr e (nbe (α ⇒' β) e)  ∧  ∀ e', R α e' → R β (e ⬝ e')
 
 -- R a e  implies  e ~ nbe a e
 lemma R_convr_nbe (h : R a e)  : convr e (nbe a e) :=
@@ -567,3 +567,4 @@ lemma convr_R_iff : ∀ e e', convr e e' → (R α e ↔ R α e') :=
         rewrite [βIH (f1 ⬝ e') (f2 ⬝ e') (f1_r_f2.app convr.refl)]
         rcases R_f2 with ⟨_, h0⟩
         exact h0 e' Re'
+-/
