lakefile.lean
@@ -13,5 +13,5 @@ require mathlib from git
   "https://github.com/leanprover-community/mathlib4.git"
 
 @[default_target]
-lean_lib «Lean4equivRw» where
+lean_lib «Tactic» where
   -- add any library configuration options here
